src/program_proof/tulip/program/replica/replica.v
@@ -1,7 +1,28 @@
 From Perennial.program_proof.tulip Require Import prelude.
+From Perennial.program_proof.tulip.invariance Require Import validate execute.
 From Perennial.program_proof.tulip.program Require Import tuple index txnlog.
 (* From Perennial.program_proof.tulip.tulip.invariance Require Import advance accept. *)
-From Goose.github_com.mit_pdos.tulip Require Import replica.
+From Goose.github_com.mit_pdos.tulip Require Import tulip replica.
+
+Inductive rpres :=
+| ReplicaOK
+| ReplicaCommittedTxn
+| ReplicaAbortedTxn
+| ReplicaStaleCoordinator
+| ReplicaFailedValidation
+| ReplicaInvalidRank
+| ReplicaWrongLeader.
+
+Definition rpres_to_u64 (r : rpres) :=
+  match r with
+  | ReplicaOK => (U64 0)
+  | ReplicaCommittedTxn => (U64 1)
+  | ReplicaAbortedTxn => (U64 2)
+  | ReplicaStaleCoordinator => (U64 3)
+  | ReplicaFailedValidation => (U64 4)
+  | ReplicaInvalidRank => (U64 5)
+  | ReplicaWrongLeader => (U64 6)
+  end.
 
 Section replica.
   Context `{!heapGS Σ, !tulip_ghostG Σ}.
@@ -73,6 +94,19 @@ Section replica.
       "%Hptsmabs"  ∷ ⌜absrel_ptsm ptsm ptsmM⌝ ∗
       "%Hsptsmabs" ∷ ⌜absrel_ptsm sptsm sptsmM⌝.
 
+  Lemma own_replica_ptsm_sptsm_dom rp ptsm sptsm :
+    own_replica_ptsm_sptsm rp ptsm sptsm -∗
+    ⌜keys_all ⊆ dom ptsm ∧ keys_all ⊆ dom sptsm⌝.
+  Proof.
+    iNamed 1.
+    iPureIntro.
+    split.
+    - intros k Hk. specialize (Hptsmabs _ Hk).
+      apply elem_of_dom. by destruct (ptsmM !! k).
+    - intros k Hk. specialize (Hsptsmabs _ Hk).
+      apply elem_of_dom. by destruct (sptsmM !! k).
+  Qed.
+
   Definition own_replica_bm_laim
     (rp : loc) (bm : gmap nat ballot) (laim : gmap nat nat) : iProp Σ :=
     (* TODO: find the right type for pstbl and the absrel. *)
@@ -80,12 +114,12 @@ Section replica.
       "HpstblP" ∷ rp ↦[Replica :: "pstbl"] #pstblP ∗
       "Hpstbl"  ∷ own_map pstblP (DfracOwn 1) pstbl.
 
-  Definition own_replica (rp : loc) (gid rid : u64) α γ : iProp Σ :=
+  Definition own_replica (rp : loc) (gid rid : u64) γ α : iProp Σ :=
     ∃ (lsna : u64) (cm : gmap nat bool) (histm : gmap dbkey dbhist)
       (cpm : gmap nat dbmap) (ptgsm : gmap nat (gset u64))
       (sptsm ptsm : gmap dbkey nat) (bm : gmap nat ballot) (laim : gmap nat nat)
-      (clog : dblog) (ilog : list (nat * icommand)),
-      let log := merge_clog_ilog clog ilog in
+      (clog cloga : dblog) (ilog : list (nat * icommand)),
+      let log := merge_clog_ilog cloga ilog in
       "Hlsna"      ∷ rp ↦[Replica :: "lsna"] #lsna ∗
       "Hcm"        ∷ own_replica_cm rp cm ∗
       "Hphistm"    ∷ ([∗ map] k ↦ h ∈ histm, own_phys_hist_half α k h) ∗
@@ -94,12 +128,15 @@ Section replica.
       "Hbmlaim"    ∷ own_replica_bm_laim rp bm laim ∗
       "Hclog"      ∷ own_replica_clog_half γ gid rid clog ∗
       "Hilog"      ∷ own_replica_ilog_half γ gid rid ilog ∗
+      "#Hrpvds"    ∷ ([∗ set] t ∈ dom cpm, is_replica_validated_ts γ gid rid t) ∗
+      "#Hclogalb"  ∷ is_txn_log_lb γ gid cloga ∗
+      "%Hcloga"    ∷ ⌜prefix clog cloga⌝ ∗
       "%Hexec"     ∷ ⌜execute_cmds log = LocalState cm histm cpm ptgsm sptsm ptsm bm laim⌝.
 
-  Definition is_replica (rp : loc) α γ : iProp Σ :=
-    ∃ (gid rid : u64) (mu : loc) (txnlog : loc) (idx : loc),
+  Definition is_replica (rp : loc) : iProp Σ :=
+    ∃ (mu : loc) (txnlog : loc) (idx : loc) (gid rid : u64) γ α,
       "#HmuP"     ∷ readonly (rp ↦[Replica :: "mu"] #mu) ∗
-      "#Hlock"    ∷ is_lock tulipNS #mu (own_replica rp gid rid α γ) ∗
+      "#Hlock"    ∷ is_lock tulipNS #mu (own_replica rp gid rid γ α) ∗
       "#HtxnlogP" ∷ readonly (rp ↦[Replica :: "txnlog"] #txnlog) ∗
       "#Htxnlog"  ∷ is_txnlog txnlog gid γ ∗
       "#HidxP"    ∷ readonly (rp ↦[Replica :: "idx"] #idx) ∗
@@ -122,7 +159,6 @@ Section replica.
     key_writable_ptsm ptsm key ∧ key_writable_sptsm sptsm ts key.
 
   Theorem wp_Replica__writableKey rp (ts : u64) key ptsm sptsm :
-    uint.Z ts ≠ 0 ->
     key ∈ keys_all ->
     {{{ own_replica_ptsm_sptsm rp ptsm sptsm }}}
       Replica__writableKey #rp #ts #(LitString key)
@@ -131,7 +167,7 @@ Section replica.
         ⌜if ok then key_writable ptsm sptsm (uint.nat ts) key else True⌝
     }}}.
   Proof.
-    iIntros (Htsnz Hkey Φ) "Hrp HΦ".
+    iIntros (Hkey Φ) "Hrp HΦ".
     wp_rec.
 
     (*@ func (rp *Replica) writableKey(ts uint64, key string) bool {            @*)
@@ -154,7 +190,6 @@ Section replica.
     (*@     spts := rp.sptsm[key]                                               @*)
 
     (*@     if ts <= spts {                                                     @*)
-
     (*@         return false                                                    @*)
     (*@     }                                                                   @*)
     (*@                                                                         @*)
@@ -191,7 +226,7 @@ Section replica.
         apply map_get_false in Hspts as [Hspts _].
         rewrite Hspts in Hsptsmabs.
         rewrite /key_writable_sptsm Hsptsmabs.
-        clear -Hgespts Htsnz. word.
+        clear -Hgespts. word.
       }
     }
     by iFrame "HptsmP HsptsmP ∗".
@@ -435,6 +470,412 @@ Section replica.
         word.
       }
     }
+  Qed.
+
+  Theorem wp_Replica__acquire rp (tsW : u64) pwrsS pwrsL pwrs ptsm sptsm :
+    valid_wrs pwrs ->
+    let ts := uint.nat tsW in
+    {{{ own_dbmap_in_slice pwrsS pwrsL pwrs ∗ own_replica_ptsm_sptsm rp ptsm sptsm }}}
+      Replica__acquire #rp #tsW (to_val pwrsS)
+    {{{ (acquired : bool), RET #acquired;
+        own_dbmap_in_slice pwrsS pwrsL pwrs ∗
+        if acquired
+        then own_replica_ptsm_sptsm rp (acquire ts pwrs ptsm) (acquire ts pwrs sptsm) ∗
+             ⌜validated_ptsm ptsm pwrs⌝ ∗
+             ⌜validated_sptsm sptsm ts pwrs⌝
+        else own_replica_ptsm_sptsm rp ptsm sptsm
+    }}}.
+  Proof.
+    iIntros (Hvw ts Φ) "[[HpwrsS %HpwrsL] Hrp] HΦ".
+    wp_rec.
+    iDestruct (own_replica_ptsm_sptsm_dom with "Hrp") as %[Hdomptsm Hdomsptsm].
+
+    (*@ func (rp *Replica) acquire(ts uint64, pwrs []tulip.WriteEntry) bool {   @*)
+    (*@     // Check if all keys are writable.                                  @*)
+    (*@     var pos uint64 = 0                                                  @*)
+    (*@                                                                         @*)
+    wp_apply (wp_ref_to); first by auto.
+    iIntros (posP) "HposP".
+    wp_pures.
+
+    (*@     for pos < uint64(len(pwrs)) {                                       @*)
+    (*@         ent := pwrs[pos]                                                @*)
+    (*@         writable := rp.writableKey(ts, ent.Key)                         @*)
+    (*@         if !writable {                                                  @*)
+    (*@             break                                                       @*)
+    (*@         }                                                               @*)
+    (*@         pos++                                                           @*)
+    (*@     }                                                                   @*)
+    (*@                                                                         @*)
+    iDestruct (own_slice_sz with "HpwrsS") as %Hlen.
+    iDestruct (own_slice_small_acc with "HpwrsS") as "[HpwrsS HpwrsC]".
+    set P := (λ (cont : bool), ∃ (pos : u64),
+      let pwrs' := list_to_map (take (uint.nat pos) pwrsL) in
+      "HpwrsS"  ∷ own_slice_small pwrsS (struct.t WriteEntry) (DfracOwn 1) pwrsL ∗
+      "HposP"   ∷ posP ↦[uint64T] #pos ∗
+      "Hrp"     ∷ own_replica_ptsm_sptsm rp ptsm sptsm ∗
+      "%Hptsm"  ∷ ⌜validated_ptsm ptsm pwrs'⌝ ∗
+      "%Hsptsm" ∷ ⌜validated_sptsm sptsm ts pwrs'⌝)%I.
+    wp_apply (wp_forBreak_cond P with "[] [HpwrsS HposP Hrp]"); last first; first 1 last.
+    { (* Loop entry. *)
+      iExists (W64 0).
+      rewrite uint_nat_W64_0 take_0 list_to_map_nil.
+      iFrame.
+      iPureIntro.
+      (* split; first done. *)
+      split.
+      { rewrite /validated_ptsm dom_empty_L.
+        intros k n Hn.
+        by apply map_lookup_filter_Some in Hn as [_ ?].
+      }
+      { rewrite /validated_sptsm dom_empty_L.
+        intros k n Hn.
+        by apply map_lookup_filter_Some in Hn as [_ ?].
+      }
+    }
+    { (* Loop body. *)
+      clear Φ. iIntros (Φ) "!> HP HΦ". iNamed "HP".
+      wp_load.
+      wp_apply (wp_slice_len).
+      wp_if_destruct; last first.
+      { (* Exit from the loop condition. *)
+        iApply "HΦ".
+        iExists pos.
+        by iFrame "∗ %".
+      }
+      wp_load.
+      destruct (lookup_lt_is_Some_2 pwrsL (uint.nat pos)) as [[k v] Hwr]; first word.
+      wp_apply (wp_SliceGet with "[$HpwrsS]"); first done.
+      iIntros "HpwrsL".
+      wp_pures.
+      wp_apply (wp_Replica__writableKey with "Hrp").
+      { rewrite -HpwrsL in Hwr.
+        apply elem_of_list_lookup_2, elem_of_map_to_list, elem_of_dom_2 in Hwr.
+        clear -Hvw Hwr. set_solver.
+      }
+      iIntros (ok) "[Hrp %Hwritable]".
+      wp_pures.
+      destruct ok; wp_pures; last first.
+      { iApply "HΦ".
+        by iFrame "∗ %".
+      }
+      wp_load.
+      wp_store.
+      iApply "HΦ".
+      iFrame "∗ %".
+      iPureIntro.
+      rewrite uint_nat_word_add_S; last word.
+      rewrite (take_S_r _ _ _ Hwr) list_to_map_snoc; last first.
+      { by eapply map_to_list_not_elem_of_take_key. }
+      split.
+      { intros x n Hn.
+        apply map_lookup_filter_Some in Hn as [Hn Hx].
+        rewrite /= dom_insert_L elem_of_union in Hx.
+        destruct Hx as [Hx | Hx]; last first.
+        { specialize (Hptsm x n). simpl in Hptsm.
+          apply Hptsm.
+          by apply map_lookup_filter_Some.
+        }
+        rewrite elem_of_singleton in Hx. subst x.
+        destruct Hwritable as [Hwritable _].
+        by rewrite /key_writable_ptsm Hn in Hwritable.
+      }
+      { intros x n Hn.
+        apply map_lookup_filter_Some in Hn as [Hn Hx].
+        rewrite /= dom_insert_L elem_of_union in Hx.
+        destruct Hx as [Hx | Hx]; last first.
+        { specialize (Hsptsm x n). simpl in Hsptsm.
+          apply Hsptsm.
+          by apply map_lookup_filter_Some.
+        }
+        rewrite elem_of_singleton in Hx. subst x.
+        destruct Hwritable as [_ Hwritable].
+        by rewrite /key_writable_sptsm Hn in Hwritable.
+      }
+    }
+    iNamed 1. clear P.
+
+    (*@     // Report error if some key cannot be locked.                       @*)
+    (*@     if pos < uint64(len(pwrs)) {                                        @*)
+    (*@         return false                                                    @*)
+    (*@     }                                                                   @*)
+    (*@                                                                         @*)
+    wp_load.
+    wp_apply wp_slice_len.
+    wp_if_destruct.
+    { iDestruct ("HpwrsC" with "HpwrsS") as "HpwrsS".
+      iApply "HΦ".
+      by iFrame "∗ %".
+    }
+    rewrite take_ge in Hptsm, Hsptsm; last word.
+    rewrite -HpwrsL list_to_map_to_list in Hptsm, Hsptsm.
+
+    (*@     // Acquire locks for each key.                                      @*)
+    (*@     for _, ent := range(pwrs) {                                         @*)
+    (*@         rp.acquireKey(ts, ent.Key)                                      @*)
+    (*@     }                                                                   @*)
+    (*@                                                                         @*)
+    set P := (λ (i : u64),
+      let pwrs' := list_to_map (take (uint.nat i) pwrsL) in
+      own_replica_ptsm_sptsm rp (acquire ts pwrs' ptsm) (acquire ts pwrs' sptsm))%I.
+    wp_apply (wp_forSlice P with "[] [$HpwrsS Hrp]"); last first; first 1 last.
+    { (* Loop entry. *)
+      subst P. simpl.
+      by rewrite uint_nat_W64_0 take_0 list_to_map_nil /acquire 2!setts_empty.
+    }
+    { (* Loop body. *)
+      clear Φ.
+      iIntros (i [k v]) "!>".
+      iIntros (Φ) "(Hrp & %Hbound & %Hi) HΦ".
+      subst P. simpl.
+      wp_pures.
+      wp_apply (wp_Replica__acquireKey with "Hrp").
+      iIntros "Hrp".
+      iApply "HΦ".
+      rewrite uint_nat_word_add_S; last word.
+      rewrite (take_S_r _ _ _ Hi) list_to_map_snoc; last first.
+      { by eapply map_to_list_not_elem_of_take_key. }
+      rewrite /acquire setts_insert; last first.
+      { rewrite -HpwrsL in Hi.
+        apply elem_of_list_lookup_2, elem_of_map_to_list, elem_of_dom_2 in Hi.
+        clear -Hvw Hi Hdomptsm. set_solver.
+      }
+      rewrite /acquire setts_insert; last first.
+      { rewrite -HpwrsL in Hi.
+        apply elem_of_list_lookup_2, elem_of_map_to_list, elem_of_dom_2 in Hi.
+        clear -Hvw Hi Hdomsptsm. set_solver.
+      }
+      done.
+    }
+    iIntros "[HP HpwrsS]".
+    iNamed "HP". clear P.
+    rewrite -Hlen firstn_all -HpwrsL list_to_map_to_list in Hptsmabs, Hsptsmabs.
+
+    (*@     return true                                                         @*)
+    (*@ }                                                                       @*)
+    wp_pures.
+    iDestruct ("HpwrsC" with "HpwrsS") as "HpwrsS".
+    iApply "HΦ".
+    by iFrame "HptsmP HsptsmP ∗ %".
+  Qed.
+
+  Theorem wp_Replica__logValidate rp (ts : u64) (pwrsS : Slice.t) (ptgsS : Slice.t) :
+    {{{ True }}}
+      Replica__logValidate #rp #ts (to_val pwrsS) (to_val ptgsS)
+    {{{ RET #(); True }}}.
+  Proof.
+    (*@ func (rp *Replica) logValidate(ts uint64, pwrs []tulip.WriteEntry, ptgs []uint64) { @*)
+    (*@     // TODO: Create an inconsistent log entry for validating @ts with @pwrs and @ptgs. @*)
+    (*@ }                                                                       @*)
+  Admitted.
+
+  Definition validate_outcome γ gid rid ts r : iProp Σ :=
+    match r with
+    | ReplicaOK => is_replica_validated_ts γ gid rid ts
+    | ReplicaCommittedTxn => (∃ wrs, is_txn_committed γ ts wrs)
+    | ReplicaAbortedTxn => is_txn_aborted γ ts
+    | ReplicaStaleCoordinator => False
+    | ReplicaFailedValidation => True
+    | ReplicaInvalidRank => False
+    | ReplicaWrongLeader => False
+    end.
+
+  Theorem wp_Replica__validate
+    rp (tsW : u64) pwrsS pwrsL pwrs (ptgsS : Slice.t) gid rid γ α :
+    let ts := uint.nat tsW in
+    gid ∈ gids_all ->
+    rid ∈ rids_all ->
+    safe_txn_pwrs γ gid ts pwrs -∗
+    know_tulip_inv γ -∗
+    {{{ own_dbmap_in_slice pwrsS pwrsL pwrs ∗ own_replica rp gid rid γ α }}}
+      Replica__validate #rp #tsW (to_val pwrsS) (to_val ptgsS)
+    {{{ (res : rpres), RET #(rpres_to_u64 res);
+        own_replica rp gid rid γ α ∗ validate_outcome γ gid rid ts res
+    }}}.
+  Proof.
+    iIntros (ts Hgid Hrid) "#Hsafepwrs #Hinv".
+    iIntros (Φ) "!> [Hpwrs Hrp] HΦ".
+    wp_rec.
+
+    (*@ func (rp *Replica) validate(ts uint64, pwrs []tulip.WriteEntry, ptgs []uint64) uint64 { @*)
+    (*@     // Check if the transaction has aborted or committed. If so, returns the @*)
+    (*@     // status immediately.                                              @*)
+    (*@     cmted, done := rp.txntbl[ts]                                        @*)
+    (*@     if done {                                                           @*)
+    (*@         if cmted {                                                      @*)
+    (*@             return tulip.REPLICA_COMMITTED_TXN                          @*)
+    (*@         } else {                                                        @*)
+    (*@             return tulip.REPLICA_ABORTED_TXN                            @*)
+    (*@         }                                                               @*)
+    (*@     }                                                                   @*)
+    (*@                                                                         @*)
+    iNamed "Hrp". iNamed "Hcm".
+    wp_loadField.
+    wp_apply (wp_MapGet with "Htxntbl").
+    iIntros (cmted bdone) "[%Hcmted Htxntbl]".
+    wp_pures.
+    destruct bdone; wp_pures.
+    { destruct cmted; wp_pures.
+      { iApply ("HΦ" $! ReplicaCommittedTxn).
+        (* Open atomic invariant to obtain [is_txn_committed]. *)
+        iInv "Hinv" as "> HinvO" "HinvC".
+        iAssert (∃ wrs, is_txn_committed γ ts wrs)%I as "#Hcmted".
+        { (* First show that [ts] is committed on the replica. *)
+          rename cm into cmrp.
+          apply map_get_true in Hcmted. symmetry in Hcmabs.
+          pose proof (lookup_kmap_eq_Some _ _ _ _ _ _ Hcmabs Hcmted) as (ts' & Hts' & Hcmrpts).
+          assert (ts' = ts) as ->.
+          { subst ts. rewrite Hts'. lia. }
+          (* Next open the group invariant to obtain [is_txn_committed]. *)
+          iNamed "HinvO".
+          unshelve epose proof (execute_cmds_apply_cmds cloga ilog cmrp histm _) as Happly.
+          { by eauto 10. }
+          iDestruct (big_sepS_elem_of with "Hgroups") as "Hgroup"; first apply Hgid.
+          do 2 iNamed "Hgroup".
+          iDestruct (txn_log_prefix with "Hlog Hclogalb") as %Hprefix.
+          pose proof (apply_cmds_mono_cm Hprefix Hrsm Happly) as Hcmrp.
+          pose proof (lookup_weaken _ _ _ _ Hcmrpts Hcmrp) as Hcmts.
+          rewrite Hcm lookup_omap_Some in Hcmts.
+          destruct Hcmts as (st & Hstcmted & Hst).
+          destruct st; [done | | done].
+          by iDestruct (big_sepM_lookup with "Hsafestm") as "Hcmted"; first apply Hst.
+        }
+        iMod ("HinvC" with "HinvO") as "_".
+        by iFrame "∗ # %".
+      }
+      { iApply ("HΦ" $! ReplicaAbortedTxn).
+        (* Open atomic invariant to obtain [is_txn_aborted]. *)
+        iInv "Hinv" as "> HinvO" "HinvC".
+        iAssert (is_txn_aborted γ ts)%I as "#Habted".
+        { (* First show that [ts] is aborted on the replica. *)
+          rename cm into cmrp.
+          apply map_get_true in Hcmted. symmetry in Hcmabs.
+          pose proof (lookup_kmap_eq_Some _ _ _ _ _ _ Hcmabs Hcmted) as (ts' & Hts' & Hcmrpts).
+          assert (ts' = ts) as ->.
+          { subst ts. rewrite Hts'. lia. }
+          (* Next open the group invariant to obtain [is_txn_aborted]. *)
+          iNamed "HinvO".
+          unshelve epose proof (execute_cmds_apply_cmds cloga ilog cmrp histm _) as Happly.
+          { by eauto 10. }
+          iDestruct (big_sepS_elem_of with "Hgroups") as "Hgroup"; first apply Hgid.
+          do 2 iNamed "Hgroup".
+          iDestruct (txn_log_prefix with "Hlog Hclogalb") as %Hprefix.
+          pose proof (apply_cmds_mono_cm Hprefix Hrsm Happly) as Hcmrp.
+          pose proof (lookup_weaken _ _ _ _ Hcmrpts Hcmrp) as Hcmts.
+          rewrite Hcm lookup_omap_Some in Hcmts.
+          destruct Hcmts as (st & Hstabted & Hst).
+          destruct st; [done | done |].
+          by iDestruct (big_sepM_lookup with "Hsafestm") as "Habted"; first apply Hst.
+        }
+        iMod ("HinvC" with "HinvO") as "_".
+        by iFrame "∗ # %".
+      }
+    }
+
+    (*@     // Check if the replica has already validated this transaction.     @*)
+    (*@     _, validated := rp.prepm[ts]                                        @*)
+    (*@     if validated {                                                      @*)
+    (*@         return tulip.REPLICA_OK                                         @*)
+    (*@     }                                                                   @*)
+    (*@                                                                         @*)
+    iNamed "Hcpm".
+    iDestruct (big_sepM2_dom with "Hprepm") as %Hdomprepm.
+    wp_loadField.
+    wp_apply (wp_MapGet with "HprepmS").
+    iIntros (prepS validated) "[%Hvalidated HprepmS]".
+    wp_pures.
+    destruct validated; wp_pures.
+    { apply map_get_true in Hvalidated.
+      iApply ("HΦ" $! ReplicaOK).
+      assert (Hin : ts ∈ dom cpm).
+      { apply elem_of_dom_2 in Hvalidated.
+        rewrite Hdomprepm elem_of_dom in Hvalidated.
+        destruct Hvalidated as [b Hb].
+        symmetry in Hcpmabs.
+        pose proof (lookup_kmap_eq_Some _ _ _ _ _ _ Hcpmabs Hb) as (ts' & Hts' & Hin).
+        assert (ts' = ts) as ->.
+        { subst ts. rewrite Hts'. lia. }
+        by apply elem_of_dom_2 in Hin.
+      }
+      iDestruct (big_sepS_elem_of with "Hrpvds") as "#Hrpvd"; first apply Hin.
+      by iFrame "∗ # %".
+    }
+
+    (*@     // Validate timestamps.                                             @*)
+    (*@     acquired := rp.acquire(ts, pwrs)                                    @*)
+    (*@     if !acquired {                                                      @*)
+    (*@         return tulip.REPLICA_FAILED_VALIDATION                          @*)
+    (*@     }                                                                   @*)
+    (*@                                                                         @*)
+    iDestruct (safe_txn_pwrs_dom_pwrs with "Hsafepwrs") as %Hdompwrs.
+    wp_apply (wp_Replica__acquire with "[$Hpwrs $Hptsmsptsm]").
+    { apply Hdompwrs. }
+    iIntros (acquired) "[Hpwrs Hptsmsptsm]".
+    wp_pures.
+    destruct acquired; wp_pures; last first.
+    { iApply ("HΦ" $! ReplicaFailedValidation). by iFrame "∗ # %". }
+    iDestruct "Hptsmsptsm" as "(Hptsmsptsm & %Hvptsm & %Hvsptsm)".
+
+    (*@     // Record the write set and the participant groups.                 @*)
+    (*@     rp.prepm[ts] = pwrs                                                 @*)
+    (*@     // rp.ptgsm[ts] = ptgs                                              @*)
+    (*@                                                                         @*)
+    wp_loadField.
+    wp_apply (wp_MapInsert with "HprepmS"); first done.
+    iIntros "HprepmS".
+    
+    (*@     // Logical action: Validate(@ts, @pwrs, @ptgs).                     @*)
+    (*@     rp.logValidate(ts, pwrs, ptgs)                                      @*)
+    (*@                                                                         @*)
+    wp_apply (wp_Replica__logValidate).
+    wp_pures.
+    iInv "Hinv" as "> HinvO" "HinvC".
+    iNamed "HinvO".
+    iDestruct (big_sepS_elem_of_acc with "Hgroups") as "[Hgroup HgroupsC]"; first apply Hgid.
+    iDestruct (big_sepS_elem_of_acc with "Hreplicas") as "[Hrg HrgsC]"; first apply Hgid.
+    iDestruct (big_sepS_elem_of_acc with "Hrg") as "[Hrp HrgC]"; first apply Hrid.
+    (* First catching up the consistent log. *)
+    destruct Hcloga as [cmdsa ->].
+    iMod (replica_inv_execute with "Hclogalb Hclog Hilog Hgroup Hrp")
+      as "(Hclog & Hilog & Hgroup & Hrp)".
+    (* Then apply the validate transition. *)
+    (* ∅ is a placeholder for participant groups. *)
+    iMod (replica_inv_validate _ _ ∅ with "Hsafepwrs Hclog Hilog Hrp")
+      as "(Hclog & Hilog & Hrp & #Hvd)".
+    { apply Hexec. }
+    { do 2 (split; first done).
+      apply map_get_false in Hvalidated as [Hnone _].
+      symmetry in Hcpmabs.
+      rewrite -not_elem_of_dom Hdomprepm not_elem_of_dom in Hnone.
+      unshelve epose proof (lookup_kmap_eq_None _ _ _ _ _ Hcpmabs Hnone) as Hcpm.
+      apply Hcpm.
+      word.
+    }
+    iDestruct ("HrgC" with "Hrp") as "Hrg".
+    iDestruct ("HrgsC" with "Hrg") as "Hrgs".
+    iDestruct ("HgroupsC" with "Hgroup") as "Hgroups".
+    iMod ("HinvC" with "[$Htxnsys $Hkeys $Hgroups $Hrgs]") as "_".
+
+    (*@     return tulip.REPLICA_OK                                             @*)
+    (*@ }                                                                       @*)
+    iApply ("HΦ" $! ReplicaOK).
+    iDestruct (big_sepM2_insert_2 _ _ _ tsW with "[Hpwrs] Hprepm") as "Hprepm".
+    { iFrame "Hpwrs". }
+    iAssert ([∗ set] t ∈ dom (<[ts := pwrs]> cpm), is_replica_validated_ts γ gid rid t)%I
+      as "Hrpvds'".
+    { rewrite dom_insert_L.
+      iApply (big_sepS_insert_2 ts with "Hvd Hrpvds").
+    }
+    iClear "Hrpvds".
+    iFrame "∗ # %".
+    iModIntro.
+    iPureIntro. simpl.
+    exists (<[ts := ∅]> ptgsm), bm, laim.
+    split.
+    { rewrite 2!kmap_insert. f_equal; [word | done]. }
+    split; first done.
+    rewrite merge_clog_ilog_snoc_ilog; last done.
+    by rewrite /execute_cmds foldl_snoc execute_cmds_unfold Hexec /=.
   Qed.
 
 End replica.
