src/program_proof/rsm/pure/fin_maps_list.v
@@ -1,0 +1,21 @@
+From iris.proofmode Require Import proofmode.
+From Perennial.program_proof.rsm.pure Require Import list.
+
+Section lemmas.
+  Context `{FinMap K M}.
+
+  Lemma map_to_list_not_elem_of_take_key {A} {m : M A} l i k v :
+    map_to_list m = l ->
+    l !! i = Some (k, v) ->
+    k ∉ (take i l).*1.
+  Proof.
+    intros Hl Hkv.
+    pose proof (NoDup_fst_map_to_list m) as Hnd.
+    rewrite Hl in Hnd.
+    pose proof (list_lookup_fmap fst l i) as Hi.
+    rewrite Hkv in Hi.
+    pose proof (not_elem_of_take _ _ _ Hnd Hi) as Htake.
+    by rewrite -fmap_take in Htake.
+  Qed.
+
+End lemmas.
